ProcessEpoch_O.thy
@@ -1,34 +1,168 @@
 theory ProcessEpoch_O
-imports Hoare_Logic
+imports Hoare_Logic "algebra/rg-algebra/General/Iteration_Liberation" ProcessEpoch
 begin
-
 
 record ProgressiveBalancesCache = 
    total_active_balance_f :: u64
    previous_epoch_flag_attesting_balances_f :: "u64 list"
    current_epoch_flag_attesting_balances_f ::  "u64 list"
 
-find_consts ProgressiveBalancesCache
-
 record ActivationQueue =
    eligible_validators_f :: "(Epoch \<times> u64) list"
 
-locale extended_vc = verified_con  +
-  fixes "progressive_balances_cache" :: 'b 
+record BaseRewardsCache = 
+  effective_balances_f :: "u64 list"
+  base_rewards_f :: "u64 list"
+
+record SlashingsContext = 
+    adjusted_total_slashing_balance_f :: "u64"
+    target_withdrawable_epoch_f :: Epoch
+
+
+record ExitCache =
+    exit_epoch_counts_f :: "Epoch \<rightharpoonup> u64"
+
+record StateContext =
+    current_epoch_f :: Epoch
+    next_epoch_f :: Epoch
+    is_in_inactivity_leak_f :: bool
+    churn_limit_f :: u64
+
+record RewardsAndPenaltiesContext =
+    unslashed_participating_increments_array_f :: "u64 list"
+    active_increments_f :: "u64"
+
+record ValidatorInfo =
+    index_f :: u64
+    effective_balance_f :: u64
+    base_reward_f :: u64
+    is_eligible_f :: bool
+    is_slashed_f :: bool
+    is_active_current_epoch_f :: bool
+    is_active_previous_epoch_f :: bool
+    previous_epoch_participation_f :: ParticipationFlags
+    current_epoch_participation_f :: ParticipationFlags
+
+record EffectiveBalancesContext = 
+    downward_threshold_f ::  u64
+    upward_threshold_f :: u64
+
+type_synonym ('e, 'addr) ref = "((BeaconState \<times> ('addr \<Rightarrow> 'addr heap_value option)), 'e option) lens"
+
+
+locale extended_vc = verified_con  + 
+  fixes "progressive_balances_cache" :: "(ProgressiveBalancesCache, 'b) ref" 
+  fixes "activation_queue" :: "(ActivationQueue, 'b) ref" 
+  fixes "state_context" :: "(StateContext, 'b) ref"
+  fixes "exit_cache" :: "(ExitCache, 'b) ref"
+  fixes "base_rewards_cache" :: "(BaseRewardsCache, 'b) ref"
+  fixes "num_active_validators" :: "(u64, 'b) ref"
+
+  assumes valid_pbc[simp]: "valid_lens progressive_balances_cache"
+  assumes valid_ac[simp]:  "valid_lens activation_queue"
+  assumes valid_sc[simp]:  "valid_lens state_context"
+  assumes valid_ec[simp]:  "valid_lens exit_cache"
+  assumes valid_brc[simp]: "valid_lens base_rewards_cache"
+  assumes valid_nav[simp]: "valid_lens num_active_validators"
+
+
+
+context verified_con begin
+
+definition "abstract R f = spec R ; f ()"
+
+definition "grab S = do {
+  _ <- assertion (\<lambda>_. S \<noteq> {});
+  angel S 
+}"
+
+
+definition "singleton_p f \<equiv> Abs_p_set (Pair {id, f} f)"
+
+
+lemma set_of_singleton [simp]: "set_of (singleton_p f) = {id, f}" 
+  apply (clarsimp simp: set_of_def singleton_p_def)
+  by (subst Abs_p_set_inverse; clarsimp)
+
+lemma point_of_singleton [simp]: "point_of (singleton_p f) = f" 
+  apply (clarsimp simp: point_of_def singleton_p_def)
+  by (subst Abs_p_set_inverse; clarsimp)
+
+term "(\<lambda>s. grab {(l, s').  ((maps_to l v -* eq (singleton_p (K s)))) s'}) "
+
+definition "alloc v f = (\<Sqinter>R. \<Squnion>l. assert (Collect (lift (maps_to l v \<longrightarrow>* R l))); spec (UNIV \<times> Collect (lift (R l))); f l)" 
+
+definition "alloc v = do {
+  s <- getState;
+  (l, s') <- grab {(l, s').  ((maps_to l v -* eq (singleton_p (K s)))) s'}; 
+  _ <- setState (set l s (Some v));
+  return l
+}"
+end
+
+
+
+context hoare_logic begin
+
+lemma drop_resource: "lift (maps_to l v \<and>* Q) s \<Longrightarrow> lift Q s"
+  apply (clarsimp simp: lift_def)
+  apply (clarsimp simp: sep_conj_def point_of_plus_domain_iff)
+  apply (rule_tac x=y in exI, clarsimp)
+  apply (clarsimp simp: maps_point_simp)
+  apply (subgoal_tac "get l s = Some v")
+   apply (subgoal_tac "get l (point_of y s) = Some v")
+  apply (clarsimp simp: sep_disj_p_set_def)
+    apply (metis maps_to_def set_get_def valid_lens_def)
+  apply (clarsimp simp: sep_disj_p_set_def)
+   apply (smt (verit, ccfv_threshold) comp_eq_elim disj_cylindric_set_def maps_to_def point_in_set set_get_def valid_lens_def)
+  by (metis get_set_def maps_to_def valid_lens_def)
+
+
+lemma "hoare_triple (ALLS l. lift (maps_to l v \<longrightarrow>* R)) (alloc v) (lift R)"
+  apply (clarsimp simp: alloc_def hoare_triple_def run_def)
+  apply (rule Inf_lower2)
+  apply (clarsimp simp: image_iff)
+   apply (rule_tac x="\<lambda>_. R" in exI)
+   apply (rule refl)
+  apply (subst Sup_le_iff, clarsimp)
+  by (metis (no_types, lifting) Collect_mono assert_iso seq_mono_left)
+
+
+lemma alloc_wp[wp]:"(\<And>l. hoare_triple (lift (P l)) (c l) Q) \<Longrightarrow>  hoare_triple (ALLS l. lift (maps_to l v \<longrightarrow>* (P l))) (bindCont (alloc v) c) (Q)"
+  apply (clarsimp simp: alloc_def hoare_triple_def run_def bindCont_def)
+  apply (rule Inf_lower2)
+  apply (clarsimp simp: image_iff)
+   apply (rule_tac x="P" in exI)
+   apply (rule refl)
+  apply (subst Sup_le_iff, clarsimp)
+  apply (rule order_trans)
+   apply (rule seq_mono_right)
+   apply (assumption)
+  apply (rule order_trans)
+   apply (rule hoare_chain')
+   apply (rule order_refl)
+  by (metis (no_types, lifting) Collect_mono assert_iso seq_mono_left)
+
+ 
+  
+
+end
+
+context extended_vc
 
 begin
 
-term "[x \<mapsto> y]"
 
-definition "maps_to x y \<equiv> \<lambda>s. s = [x \<mapsto> y]"
+text \<open>definition "maps_to x y \<equiv> \<lambda>s. snd s = [x \<mapsto> y]"
 
 term "(maps_to addr (list [ptr total_active_balance,
                            ptr previous_epoch_flag_attesting_balances,
-                           ptr current_epoch_flag_attesting_balances]) \<and>*  maps_to total_active_balance (u64 (total_active_balance_f cache)))"
+                           ptr current_epoch_flag_attesting_balances]) \<and>*  maps_to total_active_balance (u64 (total_active_balance_f cache)))"\<close>
 
-definition "translate_ProgressiveBalancesCache" :: 
-    "'b \<Rightarrow> ProgressiveBalancesCache \<Rightarrow> (('b \<Rightarrow> 'b heap_value option) \<Rightarrow> bool)"
-where "translate_ProgressiveBalancesCache addr cache s \<equiv> 
+
+text \<open>definition "translate_ProgressiveBalancesCache" :: 
+    "'b \<Rightarrow> ProgressiveBalancesCache \<Rightarrow> ('e :: stronger_sep_algebra \<times> ('b \<Rightarrow> 'b heap_value option) \<Rightarrow> bool)"
+where "translate_ProgressiveBalancesCache addr cache \<equiv> \<lambda>s.
         \<exists>total_active_balance previous_epoch_flag_attesting_balances
          current_epoch_flag_attesting_balances.
          (maps_to addr (list [ptr total_active_balance,
@@ -37,6 +171,133 @@ where "translate_ProgressiveBalancesCache addr cache s \<equiv>
           maps_to total_active_balance (u64 (total_active_balance_f cache)) \<and>* 
           maps_to previous_epoch_flag_attesting_balances ((list o map u64 o previous_epoch_flag_attesting_balances_f) cache) \<and>*
           maps_to current_epoch_flag_attesting_balances ((list o map u64 o current_epoch_flag_attesting_balances_f) cache)) s"
+
+definition "translate_ExitCache" :: 
+    "'b \<Rightarrow> ExitCache \<Rightarrow> ('e :: stronger_sep_algebra \<times> ('b \<Rightarrow> 'b heap_value option) \<Rightarrow> bool)"
+where "translate_ExitCache addr cache \<equiv> \<lambda>s.
+        (maps_to addr ((list o map u64 o exit_epoch_counts_f) cache)) s"
+
+
+definition "translate_ActivationQueue" :: 
+    "'b \<Rightarrow> ActivationQueue \<Rightarrow> ('e :: stronger_sep_algebra \<times> ('b \<Rightarrow> 'b heap_value option) \<Rightarrow> bool)"
+    where "translate_ActivationQueue addr queue \<equiv> 
+         maps_to addr (list (map (\<lambda>x. list [(u64 o raw_epoch o fst) x, u64 (snd x)]) (eligible_validators_f queue)  ))"
+
+
+definition "translate_BaseRewardsCache" :: 
+    "'b \<Rightarrow> BaseRewardsCache \<Rightarrow> ('e :: stronger_sep_algebra \<times> ('b \<Rightarrow> 'b heap_value option) \<Rightarrow> bool)"
+    where "translate_BaseRewardsCache addr cache \<equiv> \<lambda>s.
+          \<exists>effective_balances base_rewards.
+         (maps_to addr (list [ptr effective_balances,
+                           ptr base_rewards]) \<and>*
+          maps_to effective_balances ((list o map u64 o effective_balances_f) cache) \<and>*
+          maps_to base_rewards ((list o map u64 o base_rewards_f) cache)) s"
+\<close>
+text 
+\<open>def new_exit_cache(state: BeaconState) -> ExitCache:
+    exit_cache = ExitCache(exit_epoch_counts={})
+    for validator in state.validators:
+        if validator.exit_epoch != FAR_FUTURE_EPOCH:
+            record_validator_exit(exit_cache, validator.exit_epoch)
+    return exit_cache
+\<close>
+
+text 
+\<open>
+def record_validator_exit(exit_cache: ExitCache, exit_epoch: Epoch):
+    if exit_epoch in exit_cache.exit_epoch_counts:
+        exit_cache.exit_epoch_counts[exit_epoch] += 1
+    else:
+        exit_cache.exit_epoch_counts[exit_epoch] = 1
+\<close>
+
+definition record_validator_exit :: "(ExitCache, 'b) ref \<Rightarrow> Epoch \<Rightarrow> (unit, 'a) cont"
+  where "record_validator_exit ec exit_epoch \<equiv> do {
+   cache <- exit_epoch_counts_f <$> read ec;
+   if exit_epoch \<in> dom cache then do {
+        x <- the (cache exit_epoch) .+ 1;
+        let cache = cache(exit_epoch \<mapsto> x);
+        ec := return (ec\<lparr> exit_epoch_counts_f := cache \<rparr>)
+   } else do {
+     let cache = cache(exit_epoch \<mapsto> 1);
+     ec := return (ec\<lparr>exit_epoch_counts_f := cache \<rparr>)
+   }
+}"
+
+definition new_exit_cache :: "(ExitCache, 'a) cont"
+  where "new_exit_cache \<equiv> do {
+   vs <- read validators; 
+   let epochs = map exit_epoch_f (var_list_inner vs);
+   let frequency = of_nat o count_list epochs;
+   return (ExitCache.fields (\<lambda>e. if frequency e = 0 then None else Some (frequency e) ))
+}"
+
+text \<open>def get_max_exit_epoch(exit_cache: ExitCache) -> Epoch:
+    if len(exit_cache.exit_epoch_counts) == 0:
+        return 0
+    else:
+        return max(exit_cache.exit_epoch_counts.keys())\<close>
+
+definition get_max_exit_epoch :: "ExitCache \<Rightarrow> Epoch"
+  where "get_max_exit_epoch cache = Max (dom (exit_epoch_counts_f cache)) " 
+
+text \<open>def get_exit_queue_churn(exit_cache: ExitCache, exit_queue_epoch: Epoch) -> uint64:
+    return exit_cache.exit_epoch_counts.get(exit_queue_epoch) or 0\<close>
+
+definition get_exit_queue_churn :: "ExitCache \<Rightarrow> Epoch \<Rightarrow> u64"
+  where "get_exit_queue_churn cache epoch = case_option 0 id (exit_epoch_counts_f cache epoch)"
+
+notation liftM (infixl "<$>" 50)
+
+definition "exit_epoch :: (Validator, Epoch) lens \<equiv> Lens exit_epoch_f (\<lambda>v e. v\<lparr>exit_epoch_f := e\<rparr>) (\<lambda>_. True)"
+definition "withdrawable_epoch :: (Validator, Epoch) lens \<equiv> Lens withdrawable_epoch_f (\<lambda>v e. v\<lparr>withdrawable_epoch_f := e\<rparr>) (\<lambda>_. True)"
+
+abbreviation (input) "mut x \<equiv> x" 
+
+definition initiate_validator_exit_fast :: "(Validator, 'b) ref \<Rightarrow> (ExitCache, 'b) ref \<Rightarrow> StateContext \<Rightarrow> (unit, 'a) cont"
+  where "initiate_validator_exit_fast validator ec state_ctxt = do{
+   let exit_epoch = mut (exit_epoch |o> validator);
+   let withdrawable_epoch = mut (withdrawable_epoch |o> validator);
+   ee <- read exit_epoch;
+   exit_cache <- read ec;     
+   _ <- when (ee = FAR_FUTURE_EPOCH) (do {
+        let max_exit_epoch_from_cache = get_max_exit_epoch(exit_cache);
+        activation_exit_epoch \<leftarrow> (compute_activation_exit_epoch (current_epoch_f state_ctxt));
+        let exit_queue_epoch = max max_exit_epoch_from_cache activation_exit_epoch;
+        let exit_queue_churn = get_exit_queue_churn exit_cache exit_queue_epoch;
+        exit_queue_epoch <- (if exit_queue_churn \<ge> churn_limit_f state_ctxt then exit_queue_epoch .+ Epoch 1 else return exit_queue_epoch);
+        _ <- (exit_epoch :=  return exit_queue_epoch);
+        _ <- (withdrawable_epoch := ee .+ Epoch (MIN_VALIDATOR_WITHDRAWABILITY_DELAY config) );
+        _ <- record_validator_exit ec exit_queue_epoch;
+        return () });
+   return ()}"
+
+
+text \<open>def initiate_validator_exit_fast(
+    validator: Validator, exit_cache: ExitCache, state_ctxt: StateContext
+):
+    # Return if validator already initiated exit
+    if validator.exit_epoch != FAR_FUTURE_EPOCH:
+        return
+
+    # Compute exit queue epoch
+    max_exit_epoch_from_cache = get_max_exit_epoch(exit_cache)
+    exit_queue_epoch = max(
+        max_exit_epoch_from_cache,
+        compute_activation_exit_epoch(state_ctxt.current_epoch),
+    )
+    exit_queue_churn = get_exit_queue_churn(exit_cache, exit_queue_epoch)
+    if exit_queue_churn >= state_ctxt.churn_limit:
+        exit_queue_epoch += Epoch(1)
+
+    # Set validator exit epoch and withdrawable epoch
+    validator.exit_epoch = exit_queue_epoch
+    validator.withdrawable_epoch = Epoch(
+        validator.exit_epoch + MIN_VALIDATOR_WITHDRAWABILITY_DELAY
+    )
+
+    # Update cache
+    record_validator_exit(exit_cache, exit_queue_epoch)\<close>
 
 definition "read_ProgressiveBalancesCache" :: 
   "'b \<Rightarrow> (ProgressiveBalancesCache, 'a) cont"
@@ -58,6 +319,261 @@ definition "read_ProgressiveBalancesCache" ::
 }"
 
 
+definition "write_ProgressiveBalancesCache" :: 
+  "'b \<Rightarrow> ProgressiveBalancesCache \<Rightarrow> (unit, 'a) cont"
+  where "write_ProgressiveBalancesCache root_addr pbc \<equiv> do {
+        ptrs \<leftarrow> read root_addr;
+        total_active_balance_ptr \<leftarrow>  index_ptr_from_list ptrs 0;
+        previous_epoch_flag_attesting_balances_ptr \<leftarrow> index_ptr_from_list ptrs 1;
+        current_epoch_flag_attesting_balances_ptr \<leftarrow>  index_ptr_from_list ptrs 2;
+        _ \<leftarrow> write_to total_active_balance_ptr (total_active_balance_f pbc);
+        _ \<leftarrow> write_to previous_epoch_flag_attesting_balances_ptr (map u64 (previous_epoch_flag_attesting_balances_f pbc)) ;
+        _ \<leftarrow> write_to current_epoch_flag_attesting_balances_ptr (map u64 (current_epoch_flag_attesting_balances_f pbc)) ;
+        return ()
+}"
+
+
+definition "read_BaseRewardsCache" :: 
+  "'b \<Rightarrow> (BaseRewardsCache, 'a) cont"
+  where "read_BaseRewardsCache root_addr \<equiv> do {
+        ptrs \<leftarrow> read root_addr;
+        effective_balances_ptr \<leftarrow>  index_ptr_from_list ptrs 0;
+        base_rewards_ptr \<leftarrow> index_ptr_from_list ptrs 1;
+        (effective_balances :: 'b heap_value list) \<leftarrow> read effective_balances_ptr;
+        (effective_balances :: u64 list) \<leftarrow> mapM (lift_option o u64_of) effective_balances;
+        (base_rewards :: 'b heap_value list) \<leftarrow> read base_rewards_ptr;
+        (base_rewards :: u64 list) \<leftarrow> mapM (lift_option o u64_of) base_rewards;
+         return
+            (BaseRewardsCache.fields
+                effective_balances 
+                base_rewards)
+}"
+
+
+definition get_cached_base_reward :: "BaseRewardsCache \<Rightarrow> u64 => (u64, 'a) cont" 
+  where "get_cached_base_reward cache index  = do {
+    _ <- assertion (\<lambda>s. index < of_nat (length (effective_balances_f cache)));
+    effective_balance_eth <- word_unsigned_div (effective_balances_f cache ! unat index) (EFFECTIVE_BALANCE_INCREMENT config); 
+    _ <- assertion (\<lambda>s. effective_balance_eth < of_nat (length (base_rewards_f cache)));
+    return (base_rewards_f cache ! unat effective_balance_eth)
+}"
+
+
+definition get_base_reward_per_increment_fast :: "ProgressiveBalancesCache \<Rightarrow> (u64, 'a) cont"
+  where "get_base_reward_per_increment_fast progressive_balances = do {
+        x <- EFFECTIVE_BALANCE_INCREMENT config .* BASE_REWARD_FACTOR config;
+        y <- integer_squareroot (total_active_balance_f progressive_balances);
+        word_unsigned_div x y    
+}"
+
+
+definition get_base_reward_fast :: "u64 \<Rightarrow> ProgressiveBalancesCache \<Rightarrow> (u64, 'a) cont"
+  where "get_base_reward_fast effective_balance progressive_balances = do {
+    increments <- word_unsigned_div effective_balance (EFFECTIVE_BALANCE_INCREMENT config);
+    base_reward_per_increment <- get_base_reward_per_increment_fast progressive_balances;
+    increments .* base_reward_per_increment
+}"
+
+
+
+definition compute_base_rewards :: "(u64 list, 'a) cont" 
+  where "compute_base_rewards = do {
+   pbc <- read_beacon progressive_balances_cache;
+   max_balance <- MAX_EFFECTIVE_BALANCE  .+ EFFECTIVE_BALANCE_INCREMENT config;
+   xs <- forM (range 0 (unat max_balance) (unat (EFFECTIVE_BALANCE_INCREMENT config))) (\<lambda>effective_balance. get_base_reward_fast (of_nat effective_balance) pbc);
+   return (xs :: u64 list)
+}"
+
+
+definition process_single_slashing :: "u64 \<Rightarrow> Validator \<Rightarrow> SlashingsContext \<Rightarrow> ProgressiveBalancesCache \<Rightarrow> (u64, 'a) cont"
+  where "process_single_slashing balance validator s_ctxt pbc = do {
+                  let slashed = Validator.slashed_f validator;
+                  if (slashed \<and> target_withdrawable_epoch_f s_ctxt = withdrawable_epoch_f validator)
+                      then do {
+                           let increment = EFFECTIVE_BALANCE_INCREMENT config;
+                           penalty_numerator <- word_unsigned_div (Validator.effective_balance_f validator) increment;
+                           penalty_numerator <- penalty_numerator .* adjusted_total_slashing_balance_f s_ctxt;
+                           penalty <- word_unsigned_div penalty_numerator (total_active_balance_f pbc);
+                           penalty <- penalty .* increment;
+                           return (balance - penalty)
+                      }
+                      else do {return balance}
+}"
+
+text \<open>*
+    balance: Gwei,
+    validator: Validator,
+    slashings_ctxt: SlashingsContext,
+    progressive_balances: ProgressiveBalancesCache,
+) -> Gwei:
+    if (
+        validator.slashed
+        and slashings_ctxt.target_withdrawable_epoch == validator.withdrawable_epoch
+    ):
+        increment = EFFECTIVE_BALANCE_INCREMENT
+        penalty_numerator = (
+            validator.effective_balance
+            // increment
+            * slashings_ctxt.adjusted_total_slashing_balance
+        )
+        penalty = (
+            penalty_numerator // progressive_balances.total_active_balance * increment
+        )
+        return saturating_sub(balance, penalty)
+    else:
+        return balance
+*\<close>
+
+
+definition "read_ActivationQueue" :: 
+    "'b \<Rightarrow> (ActivationQueue, 'a) cont"
+    where "read_ActivationQueue addr \<equiv> do {
+         (queue :: 'b heap_value list) <- read_list addr;
+         queue' <- forM queue (\<lambda>v. do {
+              pair    <- lift_option (list_of v); 
+              epoch   <- index_u64_from_list pair 0;
+              v_index <- index_u64_from_list pair 1;
+              return (Epoch epoch, v_index)
+         });
+         return (ActivationQueue.fields queue')
+}"
+
+definition "could_be_eligible_for_activation_at" :: "Validator \<Rightarrow> Epoch \<Rightarrow> bool"
+  where "could_be_eligible_for_activation_at v e \<equiv>
+        activation_eligibility_epoch_f v < e \<and> activation_epoch_f v = FAR_FUTURE_EPOCH"
+
+definition add_if_could_be_eligible_for_activation :: "ActivationQueue \<Rightarrow> u64 \<Rightarrow> Validator \<Rightarrow> Epoch \<Rightarrow> ActivationQueue"
+  where "add_if_could_be_eligible_for_activation q i v e \<equiv> if could_be_eligible_for_activation_at v e 
+                                                             then ( q\<lparr>eligible_validators_f := (activation_eligibility_epoch_f v, i) # eligible_validators_f q\<rparr>)
+                                                             else q"
+
+
+definition new_activation_queue :: "(ActivationQueue, 'a) cont"
+  where "new_activation_queue = do {
+         current_epoch <- get_current_epoch;
+         next_epoch    <- current_epoch .+ (Epoch 1);
+         validators <- read validators;
+         let queue = fold (\<lambda>(i, v) q. add_if_could_be_eligible_for_activation q i v next_epoch) (enumerate (var_list_inner validators)) (ActivationQueue.fields []);
+         return queue }"
+
+
+text \<open>def get_validators_eligible_for_activation(
+    activation_queue: ActivationQueue,
+    finalized_epoch: Epoch,
+    churn_limit: uint64,
+) -> [ValidatorIndex]:
+    return [
+        index for (eligibility_epoch, index) in activation_queue.eligible_validators
+        if eligibility_epoch <= finalized_epoch
+    ][:churn_limit]\<close>
+
+definition get_validators_eligible_for_activation :: "ActivationQueue \<Rightarrow> Epoch \<Rightarrow> u64 \<Rightarrow> u64 list"
+  where "get_validators_eligible_for_activation queue final_epoch churn_limit \<equiv> 
+  take (unat churn_limit) (map snd (filter (\<lambda>(eligibility_epoch, index). eligibility_epoch \<le> final_epoch) (eligible_validators_f queue) ))"
+
+
+text \<open>for flag_index in range(len(participation_flag_weights)):
+        if has_flag(current_epoch_participation, flag_index):
+            if new_effective_balance > old_effective_balance:
+                next_epoch_progressive_balances.previous_epoch_flag_attesting_balances[
+                    flag_index
+                ] += (new_effective_balance - old_effective_balance)
+            else:
+                next_epoch_progressive_balances.previous_epoch_flag_attesting_balances[
+                    flag_index
+                ] -= (old_effective_balance - new_effective_balance)
+\<close>
+
+text \<open>def new_next_epoch_progressive_balances(
+    progressive_balances: ProgressiveBalancesCache,
+) -> ProgressiveBalancesCache:
+    # Set total active balance to 0, it will be updated in
+    # `process_single_effective_balance_update`.
+    total_active_balance = 0
+
+    # Rotate current epoch to previous, and initialize current to 0.
+    previous_epoch_flag_attesting_balances = (
+        progressive_balances.current_epoch_flag_attesting_balances
+    )
+    current_epoch_flag_attesting_balances = [0, 0, 0]
+
+    return ProgressiveBalancesCache(
+        total_active_balance=total_active_balance,
+        previous_epoch_flag_attesting_balances=previous_epoch_flag_attesting_balances,
+        current_epoch_flag_attesting_balances=current_epoch_flag_attesting_balances,
+    )\<close>
+
+
+definition "new_next_epoch_progressive_balance" :: "ProgressiveBalancesCache \<Rightarrow> ProgressiveBalancesCache"
+  where "new_next_epoch_progressive_balance pbc \<equiv> let 
+         new_balance = 0;
+         new_previous_epoch_flag_attesting_balances = current_epoch_flag_attesting_balances_f pbc;
+         new_current_epoch_flag_attesting_balances = [0,0,0] in
+         pbc\<lparr>total_active_balance_f := new_balance,
+             previous_epoch_flag_attesting_balances_f := new_previous_epoch_flag_attesting_balances,
+             current_epoch_flag_attesting_balances_f := new_current_epoch_flag_attesting_balances\<rparr>"
+
+definition update_next_epoch_progressive_balances :: 
+  "Epoch \<Rightarrow> (ProgressiveBalancesCache, 'b) ref \<Rightarrow> Validator \<Rightarrow> ParticipationFlags \<Rightarrow> u64 \<Rightarrow> (unit, 'a) cont"
+  where "update_next_epoch_progressive_balances next_epoch next_epoch_progressive_balances
+                               validator cep old_effective_balance = do {
+                                    let new_effective_balance = Validator.effective_balance_f validator;
+                                    total_active_balance <- total_active_balance_f <$> read next_epoch_progressive_balances;
+                                    total_active_balance <- if (is_active_validator validator next_epoch) 
+                                                                then total_active_balance .+ new_effective_balance
+                                                                else return total_active_balance;
+                                    _ <- (next_epoch_progressive_balances := return (next_epoch_progressive_balances\<lparr>total_active_balance_f := total_active_balance\<rparr>));
+                                    let flag_indexes = range 0 (length (participation_flag_weights cep)) 1; 
+                                    _ <- when (\<not> (slashed_f validator)) (do {
+                                           xs <- (if (new_effective_balance > old_effective_balance) 
+                                                      then do {
+                                                            x  <- new_effective_balance .- old_effective_balance;
+                                                            xs <- forM flag_indexes (\<lambda>i. do { ys <- previous_epoch_flag_attesting_balances_f <$> read next_epoch_progressive_balances;
+                                                                                              if (has_flag cep i) then (word_unsigned_add (ys ! i)  x)
+                                                                                                             else (return (ys ! i))});
+                                                            return xs}
+                                                      else do {
+                                                            x <- old_effective_balance .- new_effective_balance;
+                                                            xs <- forM flag_indexes (\<lambda>i. do { ys <- previous_epoch_flag_attesting_balances_f <$> read next_epoch_progressive_balances;
+                                                                                              if (has_flag cep i) then (ys ! i) .- x
+                                                                                                                  else (return (ys ! i ))});
+                                                            return xs});                                      
+                                         (next_epoch_progressive_balances := return (next_epoch_progressive_balances\<lparr>previous_epoch_flag_attesting_balances_f := xs\<rparr>))
+                                          });
+                                    return ()
+                               }"
+
+text \<open>def update_next_epoch_progressive_balances(
+    next_epoch: Epoch,
+    next_epoch_progressive_balances: ProgressiveBalancesCache,
+    validator: Validator,
+    current_epoch_participation: ParticipationFlags,
+    old_effective_balance: uint64,
+):
+    new_effective_balance = validator.effective_balance
+
+    # Update total active balance.
+    if is_active_validator(validator, next_epoch):
+        next_epoch_progressive_balances.total_active_balance += new_effective_balance
+
+    # Update the current epoch totals which are the *previous* epoch totals in the cache
+    # and were computed with the validator's `old_effective_balance`.
+    # Slashed validators are not part of the unslashed participating totals.
+    if validator.slashed:
+        return
+
+    for flag_index in range(len(participation_flag_weights)):
+        if has_flag(current_epoch_participation, flag_index):
+            if new_effective_balance > old_effective_balance:
+                next_epoch_progressive_balances.previous_epoch_flag_attesting_balances[
+                    flag_index
+                ] += (new_effective_balance - old_effective_balance)
+            else:
+                next_epoch_progressive_balances.previous_epoch_flag_attesting_balances[
+                    flag_index
+                ] -= (old_effective_balance - new_effective_balance)\<close>
+
+
 definition "process_justification_and_finalization_fast" ::  "(unit, 'a) cont"
   where "process_justification_and_finalization_fast \<equiv> do {
      previous_epoch <- get_previous_epoch;
@@ -66,7 +582,7 @@ definition "process_justification_and_finalization_fast" ::  "(unit, 'a) cont"
     if current_epoch \<le> epoch1 then
       return ()
     else do {
-      pbc \<leftarrow> read_ProgressiveBalancesCache progressive_balances_cache;
+      pbc \<leftarrow> read progressive_balances_cache;
       let (total_active_balance) = total_active_balance_f pbc;
       let (previous_epoch_flag_attesting_balances) = previous_epoch_flag_attesting_balances_f pbc;
       let (previous_target_balance) = previous_epoch_flag_attesting_balances ! (of_nat TIMELY_TARGET_FLAG_INDEX);
@@ -77,6 +593,567 @@ definition "process_justification_and_finalization_fast" ::  "(unit, 'a) cont"
       return ()
       
 }}"
+
+definition new_progressive_balances :: "(ProgressiveBalancesCache, 'a) cont"
+  where  "new_progressive_balances = return (undefined :: ProgressiveBalancesCache)"
+
+definition new_base_rewards_cache :: "(BaseRewardsCache, 'a) cont" 
+  where "new_base_rewards_cache    = return (undefined :: BaseRewardsCache)"
+
+definition get_validator_churn_limit_fast :: "(u64, 'a) cont" 
+  where "get_validator_churn_limit_fast = undefined"
+
+definition new_state_context :: "(StateContext, 'a) cont"
+  where "new_state_context = do {
+    current_epoch <- get_current_epoch;
+    next_epoch <- current_epoch .+ (Epoch 1); 
+    is_in_inactivity_leak <- is_in_inactivity_leak;
+    churn_limit <- get_validator_churn_limit_fast;
+    return (StateContext.fields current_epoch next_epoch is_in_inactivity_leak churn_limit)
+}"
+
+definition new_slashings_context :: "StateContext \<Rightarrow> (SlashingsContext, 'a) cont"
+ where "new_slashings_context = undefined"
+
+definition new_rewards_and_penalties_context :: "ProgressiveBalancesCache \<Rightarrow> (RewardsAndPenaltiesContext, 'a) cont"
+  where "new_rewards_and_penalties_context = undefined"
+
+definition new_effective_balances_ctxt :: "(EffectiveBalancesContext, 'a) cont"
+  where "new_effective_balances_ctxt = undefined"
+
+definition new_next_epoch_progressive_balances :: "ProgressiveBalancesCache \<Rightarrow> (ProgressiveBalancesCache, 'a) cont"
+  where "new_next_epoch_progressive_balances progressive_balances = undefined"
+
+definition "activation_epoch :: (Validator, Epoch) lens \<equiv>
+             Lens activation_epoch_f (\<lambda>v e. v\<lparr>activation_epoch_f := e\<rparr>) (\<lambda>_. True)"
+
+definition "v_list_lens i \<equiv> 
+            (Lens (\<lambda>l. var_list_inner l ! u64_to_nat i) (\<lambda>l e. VariableList (list_update (var_list_inner l) (u64_to_nat i) e)) (\<lambda>_. True))"
+
+definition "var_list_index_lens ls i \<equiv> do {
+  l <- read ls;
+  (if (i < var_list_len l) then return (v_list_lens i |o> ls)
+  else fail) }"
+
+notation "var_list_index_lens" (infixr "!?"  88)
+
+definition process_single_registry_update :: "(Validator, 'b) ref \<Rightarrow> ValidatorInfo \<Rightarrow> ExitCache \<Rightarrow>
+                                               u64 list \<Rightarrow> (ActivationQueue, 'b) ref \<Rightarrow> StateContext \<Rightarrow> (unit, 'a) cont"
+  where "process_single_registry_update vref val_info ex_cache aq 
+                                         next_epoch_aq state_ctxt \<equiv> do {
+      let current_epoch = current_epoch_f state_ctxt;
+      validator <- read vref;
+      _ <- when (is_eligible_for_activation_queue validator) (do {
+                 epoch <- current_epoch .+ (Epoch 1);
+                (vref := return (validator\<lparr>activation_eligibility_epoch_f := epoch\<rparr>)) 
+            });
+      validator <- read vref;
+      _ <- when (is_active_validator validator current_epoch \<and> Validator.effective_balance_f validator \<le> EJECTION_BALANCE config) 
+                (initiate_validator_exit_fast vref exit_cache state_ctxt);
+      _ <- when (index_f val_info \<in> List.set aq) (do {
+            let validator_activation_epoch = mut (activation_epoch |o> vref);
+            (validator_activation_epoch := compute_activation_exit_epoch current_epoch)
+            });
+      _ <- (next_epoch_aq := return (add_if_could_be_eligible_for_activation next_epoch_aq (index_f val_info) validator (next_epoch_f state_ctxt)));
+      return ()
+}"
+
+text \<open>
+def process_single_registry_update(
+    validator: Validator,
+    validator_info: ValidatorInfo,
+    exit_cache: ExitCache,
+    activation_queue: [ValidatorIndex],
+    next_epoch_activation_queue: ActivationQueue,
+    state_ctxt: StateContext,
+):
+    current_epoch = state_ctxt.current_epoch
+
+    if is_eligible_for_activation_queue(validator):
+        validator.activation_eligibility_epoch = current_epoch + 1
+
+    if (
+        is_active_validator(validator, current_epoch)
+        and validator.effective_balance <= EJECTION_BALANCE
+    ):
+        initiate_validator_exit_fast(validator, exit_cache, state_ctxt)
+
+    if validator_info.index in activation_queue:
+        validator.activation_epoch = compute_activation_exit_epoch(current_epoch)
+
+    # Caching: add to speculative activation queue for next epoch.
+    add_if_could_be_eligible_for_activation(
+        new_activation_queue,
+        validator_info.index,
+        validator,
+        state_ctxt.next_epoch,
+    )
+\<close>
+
+definition "is_unslashed_participating_index v_info flag_index \<equiv> 
+        is_active_previous_epoch_f v_info \<and> 
+       \<not>is_slashed_f v_info               \<and>
+        has_flag (previous_epoch_participation_f v_info) flag_index"
+
+text \<open>
+def is_unslashed_participating_index(
+    validator_info: ValidatorInfo, flag_index: int
+) -> bool:
+    return (
+        validator_info.is_active_previous_epoch
+        and not validator_info.is_slashed
+        and has_flag(validator_info.previous_epoch_participation, flag_index)
+    )
+\<close>
+definition "get_flag_index_delta v_info flag_index rewards_ctxt state_ctxt = do{
+      let base_reward = base_reward_f v_info;
+      let weight = PARTICIPATION_FLAG_WEIGHTS ! flag_index;
+      let unslashed_participating_increments = unslashed_participating_increments_array_f rewards_ctxt ! flag_index;
+      if (is_unslashed_participating_index v_info flag_index) \<and>
+                          \<not>(is_in_inactivity_leak_f state_ctxt) then do {
+          return (0,0)}
+      else if (flag_index \<noteq> TIMELY_HEAD_FLAG_INDEX) then do {
+          return (0,0)
+      } else       
+      return (0,0)
+}"
+
+text \<open>
+def get_flag_index_delta(
+    validator_info: ValidatorInfo,
+    flag_index: int,
+    rewards_ctxt: RewardsAndPenaltiesContext,
+    state_ctxt: StateContext,
+) -> (Gwei, Gwei):
+    base_reward = validator_info.base_reward
+    weight = PARTICIPATION_FLAG_WEIGHTS[flag_index]
+    unslashed_participating_increments = (
+        rewards_ctxt.unslashed_participating_increments_array[flag_index]
+    )
+
+    if is_unslashed_participating_index(validator_info, flag_index):
+        if not state_ctxt.is_in_inactivity_leak:
+            reward_numerator = base_reward * weight * unslashed_participating_increments
+            reward_denominator = rewards_ctxt.active_increments * WEIGHT_DENOMINATOR
+            reward = reward_numerator / reward_denominator
+            return (reward, 0)
+    elif flag_index != TIMELY_HEAD_FLAG_INDEX:
+        penalty = base_reward * weight / WEIGHT_DENOMINATOR
+        return (0, penalty)
+    return (0, 0)
+\<close>
+
+definition "get_inactivity_penalty_delta v_info inactivity_score state_ctxt = do {
+   if \<not>(is_unslashed_participating_index v_info TIMELY_TARGET_FLAG_INDEX) then do {
+     penalty_numerator <- effective_balance_f v_info .* inactivity_score;
+     penalty_denominator <- INACTIVITY_SCORE_BIAS config .* INACTIVITY_PENALTY_QUOTIENT_ALTAIR;
+     penalty <- word_unsigned_div penalty_numerator penalty_denominator;
+     return (0, penalty)
+   } else do {
+     return (0, 0)
+   }
+}"
+
+text \<open>def get_inactivity_penalty_delta(
+    validator_info: ValidatorInfo,
+    inactivity_score: uint64,
+    state_ctxt: StateContext,
+) -> (Gwei, Gwei):
+    # Implementation note: could abstract over fork's inactivity penalty quotient here
+    if not is_unslashed_participating_index(validator_info, TIMELY_TARGET_FLAG_INDEX):
+        penalty_numerator = validator_info.effective_balance * inactivity_score
+        penalty_denominator = INACTIVITY_SCORE_BIAS * INACTIVITY_PENALTY_QUOTIENT_BELLATRIX
+        penalty = penalty_numerator / penalty_denominator
+        return (0, penalty)
+    return (0, 0)\<close>
+
+definition ref_unsigned_add :: "(u64, 'b) ref \<Rightarrow> (u64, 'b) ref \<Rightarrow> (u64, 'a) cont" 
+  where  "ref_unsigned_add x y \<equiv> do {(x' :: u64) <- read x; (y' :: u64) <- read y;  x' .+ y'}" 
+
+definition ref_unsigned_add_l :: "u64 \<Rightarrow> (u64, 'b) ref \<Rightarrow> (u64, 'a) cont" 
+  where  "ref_unsigned_add_l x y \<equiv> do {(y' :: u64) <- read_beacon y;  x .+ y'}" 
+
+definition ref_unsigned_add_r :: "(u64, 'b) ref \<Rightarrow> u64 \<Rightarrow> (u64, 'a) cont" 
+  where  "ref_unsigned_add_r x y \<equiv> do {(x' :: u64) <- read_beacon x;  x' .+ y}" 
+
+adhoc_overloading
+  unsigned_add ref_unsigned_add ref_unsigned_add_l ref_unsigned_add_r
+
+definition "saturating_sub x y \<equiv> if x \<ge> y then x - y else 0"
+
+definition process_single_reward_and_penalty :: 
+  "u64 \<Rightarrow> u64 \<Rightarrow> ValidatorInfo \<Rightarrow> RewardsAndPenaltiesContext \<Rightarrow> StateContext \<Rightarrow> (u64, 'a) cont"
+  where "process_single_reward_and_penalty balance inactivity_score 
+                                           val_info rewards_ctxt state_ctxt \<equiv> do{
+        if (is_eligible_f val_info) then do {
+           rewards <- alloc (0 :: u64);
+           penalties <- alloc (0 :: u64);
+           let n = length PARTICIPATION_FLAG_WEIGHTS;
+           _ <- forM (range 0 n 1) (\<lambda>flag_index. do {
+             (reward,penalty) <- get_flag_index_delta val_info flag_index rewards_ctxt state_ctxt;
+             _ <- (rewards := rewards .+ reward);
+             (penalties := penalties .+ penalty)
+             });
+           (reward, penalty) <-  get_inactivity_penalty_delta val_info inactivity_score state_ctxt;
+           _ <- (rewards := rewards .+ reward);
+           _ <- (penalties := penalties .+ penalty);
+           r <- read rewards;
+           p <- read penalties;
+           (if (r \<noteq> 0 \<or> p \<noteq> 0) then do {
+               new_balance <- balance .+ r;
+               let new_balance = (if new_balance \<ge> p then new_balance - p else 0);
+               return new_balance
+           } else return balance)
+        } else (return balance)
+}"
+  
+ 
+
+text \<open>def process_single_reward_and_penalty(
+    balance: Gwei,
+    inactivity_score: uint64,
+    validator_info: ValidatorInfo,
+    rewards_ctxt: RewardsAndPenaltiesContext,
+    state_ctxt: StateContext,
+) -> uint64:
+    if not validator_info.is_eligible:
+        return balance
+
+    rewards = 0
+    penalties = 0
+
+    for flag_index in range(len(PARTICIPATION_FLAG_WEIGHTS)):
+        reward, penalty = get_flag_index_delta(
+            validator_info, flag_index, rewards_ctxt, state_ctxt
+        )
+        rewards += reward
+        penalties += penalty
+
+    reward, penalty = get_inactivity_penalty_delta(
+        validator_info,
+        inactivity_score,
+        state_ctxt,
+    )
+    rewards += reward
+    penalties += penalty
+
+    if rewards != 0 or penalties != 0:
+        new_balance = balance + rewards
+        new_balance = saturating_sub(new_balance, penalties)
+        return new_balance
+    else:
+        return balance
+\<close>
+
+definition process_single_inactivity_update :: "u64 \<Rightarrow> ValidatorInfo \<Rightarrow> StateContext \<Rightarrow> (u64, 'a) cont"
+  where "process_single_inactivity_update inactivity_score val_info state_ctxt = do {
+  if \<not>(is_eligible_f val_info) then do {
+    return inactivity_score
+  } else do {
+  let new_inactivity_score = inactivity_score;
+  new_inactivity_score <- if (is_unslashed_participating_index val_info TIMELY_TARGET_FLAG_INDEX)
+                           then (new_inactivity_score .- (min new_inactivity_score 1))
+                           else (new_inactivity_score .+ INACTIVITY_SCORE_BIAS config);
+  new_inactivity_score <- if \<not>(is_in_inactivity_leak_f state_ctxt)
+                           then (new_inactivity_score .- (min new_inactivity_score (INACTIVITY_SCORE_RECOVERY_RATE config)))
+                           else (return new_inactivity_score);
+  return new_inactivity_score
+}}"
+
+
+text \<open>def process_single_inactivity_update(
+    inactivity_score: uint64,
+    validator_info: ValidatorInfo,
+    state_ctxt: StateContext,
+) -> uint64:
+    if not validator_info.is_eligible:
+        return inactivity_score
+
+    # Increase inactivity score of inactive validators
+    new_inactivity_score = inactivity_score
+    if is_unslashed_participating_index(validator_info, TIMELY_TARGET_FLAG_INDEX):
+        new_inactivity_score -= min(1, inactivity_score)
+    else:
+        new_inactivity_score += INACTIVITY_SCORE_BIAS
+
+    # Decrease the inactivity score of all eligible validators during a leak-free epoch
+    if not state_ctxt.is_in_inactivity_leak:
+        new_inactivity_score -= min(
+            INACTIVITY_SCORE_RECOVERY_RATE, new_inactivity_score
+        )
+
+    return new_inactivity_score\<close>
+
+definition
+  process_single_effective_balance_update :: "u64 \<Rightarrow> (Validator, 'b) ref \<Rightarrow> ValidatorInfo \<Rightarrow> 
+                                             ProgressiveBalancesCache \<Rightarrow> BaseRewardsCache \<Rightarrow>
+                                             EffectiveBalancesContext \<Rightarrow> StateContext \<Rightarrow> (unit, 'a) cont"
+  where "process_single_effective_balance_update balance validator 
+                   val_info next_epb next_ebrc eb_ctxt state_ctxt = do {
+   
+  return ()
+}"
+
+text \<open>def process_single_effective_balance_update(
+    balance: Gwei,
+    validator: Validator,
+    validator_info: ValidatorInfo,
+    next_epoch_progressive_balances: ProgressiveBalancesCache,
+    next_epoch_base_reward_cache: BaseRewardCache,
+    eb_ctxt: EffectiveBalancesContext,
+    state_ctxt: StateContext,
+):
+    # Compute the effective balance change.
+    balance = state.balances[index]
+    if (
+        balance + eb_ctxt.downward_threshold < validator.effective_balance
+        or validator.effective_balance + eb_ctxt.upward_threshold < balance
+    ):
+        validator.effective_balance = min(
+            balance - balance % EFFECTIVE_BALANCE_INCREMENT, MAX_EFFECTIVE_BALANCE
+        )
+
+    # Update the progressive balances cache for the next epoch.
+    update_next_epoch_progressive_balances(
+        state_ctxt.next_epoch,
+        next_epoch_progressive_balances,
+        validator,
+        current_epoch_participation,
+        validator_info.effective_balance,
+    )
+    # Add the validator's effective balance to the base reward cache.
+    next_epoch_base_reward_cache.effective_balances.append(validator.effective_balance)\<close>
+
+definition "is_active_next_epoch (validator :: Validator) (epoch :: Epoch) = undefined"
+
+definition process_epoch_single_pass :: "(unit, 'a) cont" 
+  where "process_epoch_single_pass = do {
+  progressive_balances <- read progressive_balances_cache;
+  state_ctxt <- new_state_context;
+  slashings_ctxt <- new_slashings_context state_ctxt;
+  rewards_ctxt <- new_rewards_and_penalties_context progressive_balances;
+  effective_balances_ctxt <- new_effective_balances_ctxt;
+  next_epoch_progressive_balances <- new_next_epoch_progressive_balances progressive_balances;
+  aq <- read activation_queue; 
+  finalised_checkpoint <- epoch_f <$> read finalized_checkpoint;
+  let final_activation_queue = get_validators_eligible_for_activation aq finalised_checkpoint (churn_limit_f state_ctxt);
+  next_epoch_activation_queue <- alloc (ActivationQueue.fields []);
+  let next_epoch_base_reward_cache = BaseRewardsCache.fields [] [];
+  next_epoch_num_active_validators <- alloc (0 :: u64);
+  current_epoch <- get_current_epoch;
+  previous_epoch <- get_previous_epoch;
+  vs <- read validators;
+  _ <- forM (range 0 (unat (var_list_len vs)) 1) (\<lambda>i. do {
+     let n = of_nat i;
+     validator <- mut (validators !? n);
+     balance   <- mut (balances !? n);
+     inactivity_score <- mut (inactivity_scores !? n);
+     prev_participation <- mut (previous_epoch_participation !? n);
+     curr_participation <- mut (current_epoch_participation !? n);
+     v <- read validator;
+     let is_active_current_epoch = is_active_validator v current_epoch;
+     let is_active_previous_epoch = is_active_validator v previous_epoch;
+     x <- previous_epoch .+ (Epoch 1);
+     let is_eligible = is_active_previous_epoch \<or> (slashed_f v \<and> x < withdrawable_epoch_f v);
+     brc <- read base_rewards_cache;
+     base_reward <- get_cached_base_reward brc n;
+     p_p <- read prev_participation;
+     c_p <- read curr_participation;
+     let validator_info = ValidatorInfo.fields n (Validator.effective_balance_f v)
+                                               base_reward is_eligible (slashed_f v) is_active_current_epoch
+                                               is_active_previous_epoch p_p c_p ;
+     _ <- when (current_epoch \<noteq> GENESIS_EPOCH) (do {
+            is <- read inactivity_score; 
+            _  <- (inactivity_score := process_single_inactivity_update is validator_info state_ctxt);
+            (balance := process_single_reward_and_penalty balance is validator_info rewards_ctxt state_ctxt)
+          });
+     ec <- read exit_cache;
+     _  <- process_single_registry_update validator validator_info ec final_activation_queue next_epoch_activation_queue state_ctxt;
+     v  <- read validator;
+     _  <- (balance := process_single_slashing balance v slashings_ctxt progressive_balances);
+     b  <- read balance; 
+     _  <- process_single_effective_balance_update b validator validator_info next_epoch_progressive_balances next_epoch_base_reward_cache effective_balances_ctxt state_ctxt;
+     v  <- read validator;
+     _  <- when (is_active_next_epoch v (next_epoch_f state_ctxt)) (next_epoch_num_active_validators := next_epoch_num_active_validators .+ 1);
+     return ()
+   });
+  _ <- (progressive_balances_cache := return next_epoch_progressive_balances);
+  _ <- (activation_queue := read next_epoch_activation_queue);
+  new_base_reward <- compute_base_rewards;
+  _ <- (base_rewards_cache := return (next_epoch_base_reward_cache\<lparr>base_rewards_f := new_base_reward\<rparr>) );
+  _ <- (num_active_validators := read next_epoch_num_active_validators);
+  return ()
+ }"
+
+
+text \<open>def process_epoch_single_pass(
+    state: BeaconState,
+) -> None:
+    progressive_balances = state.progressive_balances
+
+    state_ctxt = StateContext(
+        current_epoch=get_current_epoch(state),
+        next_epoch=get_current_epoch(state) + 1,
+        is_in_inactivity_leak=is_in_inactivity_leak(state),
+        churn_limit=get_validator_churn_limit_fast(state),
+    )
+    slashings_ctxt = new_slashings_context(state, state_ctxt)
+    rewards_ctxt = new_rewards_and_penalties_context(progressive_balances)
+    effective_balances_ctxt = new_effective_balances_ctxt()
+    next_epoch_progressive_balances = new_next_epoch_progressive_balances(progressive_balances)
+
+    # Determine the final activation queue.
+    activation_queue = get_validators_eligible_for_activation(
+        state.activation_queue,
+        state.finalized_checkpoint.epoch,
+        state_ctxt.churn_limit,
+    )
+    # Create a new speculative activation queue for next epoch.
+    next_epoch_activation_queue = ActivationQueue(eligible_validators=[])
+    # Create a new base reward cache for next epoch.
+    next_epoch_base_reward_cache = BaseRewardCache(effective_balances=[], base_rewards=[])
+    # Track the number of active validators for the next epoch.
+    next_epoch_num_active_validators = 0
+
+    for (
+        index,
+        validator,
+        balance,
+        inactivity_score,
+        prev_participation,
+        curr_participation,
+    ) in zip(
+        range(0, len(state.validators)),
+        state.validators,
+        state.balances,
+        state.inactivity_scores,
+        state.previous_epoch_participation,
+        state.current_epoch_participation,
+    ):
+        is_active_current_epoch = is_active_validator(validator, current_epoch)
+        is_active_previous_epoch = is_active_validator(validator, previous_epoch)
+        is_eligible = is_active_previous_epoch or (
+            validator.slashed and previous_epoch + 1 < validator.withdrawable_epoch
+        )
+        validator_info = ValidatorInfo(
+            index=index,
+            effective_balance=validator.effective_balance,
+            base_reward=get_cached_base_reward(base_reward_cache, index),
+            is_eligible=is_eligible,
+            is_active_current_epoch=is_active_current_epoch,
+            is_active_previous_epoch=is_active_previous_epoch,
+            previous_epoch_participation=prev_participation,
+            current_epoch_participation=curr_participation
+        )
+
+        if current_epoch != GENESIS_EPOCH:
+            # Note: we may change the presentation of this mutation. Due to primitive types
+            # being immutable in Python we cannot pass a mutable reference. Our Isabelle
+            # formalisation will likely model the mutation natively (a write to the heap).
+            inactivity_score = process_single_inactivity_update(
+                inactivity_score,
+                validator_info,
+                state_ctxt,
+            )
+            state.inactivity_scores[index] = inactivity_score
+
+            balance = process_single_reward_and_penalty(
+                balance,
+                inactivity_score,
+                validator_info,
+                rewards_ctxt,
+                state_ctxt
+            )
+            state.balances[index] = balance
+
+        process_single_registry_update(
+            validator,
+            validator_info,
+            state.exit_cache,
+            activation_queue,
+            next_epoch_activation_queue,
+            state_ctxt,
+        )
+
+        balance = process_single_slashing(
+            balance,
+            validator,
+            slashings_ctxt,
+            progressive_balances,
+        )
+        state.balances[index] = balance
+
+        process_single_effective_balance_update(
+            balance,
+            validator,
+            validator_info,
+            next_epoch_progressive_balances,
+            effective_balances_ctxt,
+            state_ctxt,
+        )
+
+        # Update num active validators.
+        if is_active_next_epoch(validator, next_epoch):
+            next_epoch_num_active_validators += 1
+
+    # Update caches for next epoch.
+    state.progressive_balances = next_epoch_progressive_balances
+    state.activation_queue = next_epoch_activation_queue
+
+    # Compute base reward cache after updating progressive balance cache.
+    next_epoch_base_reward_cache.base_rewards = compute_base_rewards(state)
+    state.base_reward_cache = next_epoch_base_reward_cache
+
+    state.num_active_validators = next_epoch_num_active_validators\<close>
+
+definition process_epoch_fast :: "(unit, 'a) cont"
+  where "process_epoch_fast \<equiv> do {
+    _ <- (progressive_balances_cache := new_progressive_balances);
+    _ <- (activation_queue := new_activation_queue);
+    _ <- (exit_cache := new_exit_cache);
+    _ <- (base_rewards_cache := new_base_rewards_cache);
+    _ <- process_justification_and_finalization_fast;
+    _ <- process_epoch_single_pass;
+    _ <- process_eth1_data_reset;
+
+    return ()
+}"
+
+
+
+text\<open>
+Overview for process_epoch_fast
+
+def process_epoch_fast(state: BeaconState) -> None:
+    # Pre-conditions (not intended to be executed by implementations).
+    assert valid_progressive_balances(state)
+    assert valid_activation_queue(state)
+    assert valid_exit_cache(state)
+    assert valid_base_reward_cache(state)
+    assert valid_num_active_validators(state)
+
+    # [CHANGED] Use the aggregate sums to compute justification and finalization.
+    process_justification_and_finalization_fast(state)
+
+    # [CHANGED] Compute the majority of processing in a single iteration, utilising the progressive
+    # balances for aggregates.
+    process_epoch_single_pass(state)
+
+    # [CHANGED] Reorder `process_eth1_data_reset` after `process_effective_balances` which is now
+    # part of `process_epoch_single_pass`.
+    process_eth1_data_reset(state)
+
+    # [UNCHANGED] These functions are unaffacted.
+    process_slashings_reset(state)
+    process_randao_mixes_reset(state)
+    process_historical_summaries_update(state)
+    process_participation_flag_updates(state)
+    process_sync_committee_updates(state)
+\<close>
+
 end
+
+
+
 
 end
