Fun_Algebra.thy
@@ -1,0 +1,90 @@
+theory Fun_Algebra imports
+  "jormungand/sep_algebra/Sep_Tactics"
+  "jormungand/Hoare_Sep_Tactics/Extended_Separation_Algebra"
+  Lens
+begin
+
+instantiation unit ::  stronger_sep_algebra begin
+
+fun sep_disj_unit :: "unit \<Rightarrow> unit \<Rightarrow> bool" where
+ "sep_disj_unit x y \<longleftrightarrow> True" 
+
+fun plus_unit :: "unit \<Rightarrow> unit \<Rightarrow> unit" where
+ "plus_unit x y = ()" 
+
+
+definition "zero_unit = ()"
+
+instance
+  by (standard, case_tac x; (clarsimp simp: zero_unit_def)?)
+ 
+
+end
+
+lemma [simp]: "None ## x" by (clarsimp simp: sep_disj_option_def)
+
+definition "add_lens l l' =  Lens (\<lambda>s. (get l s, get l' s)) (\<lambda>s (a, b). set l' (set l s a) b) (\<lambda>(a, b). valid l a \<and> valid l' b)"
+
+definition "disj_lens l l' \<equiv> (\<forall>s v. get l s = get l (set l' s v)) \<and> (\<forall>s v. get l' s = get l' (set l s v)) " 
+
+definition "ptr_lens p = Lens (\<lambda>s. s p) (\<lambda>s v. s(p := v)) (\<lambda>s. True)" 
+
+lemma "p \<noteq> p' \<Longrightarrow> disj_lens (ptr_lens p) (ptr_lens p')"
+  apply (clarsimp simp: disj_lens_def, safe; clarsimp simp: ptr_lens_def)
+  done
+
+
+definition "disj_cylindric_set S S' \<equiv> \<forall>f\<in>S. \<forall>f'\<in>S'. f o f' = f' o f"
+
+
+datatype 'a domain_pair = Pair (dom_funs : "('a \<Rightarrow> 'a) set") (state_of:  "'a \<Rightarrow> 'a")
+
+abbreviation "pointed_set \<equiv> {d. state_of d \<in> dom_funs d \<and> id \<in> dom_funs d}"
+
+typedef ('a) p_set = "pointed_set :: 'a domain_pair set"
+  by (rule_tac x="Pair {id} id" in exI, clarsimp)
+
+definition "point_of p = state_of (Rep_p_set p)"
+
+definition "set_of p = dom_funs (Rep_p_set p)"
+
+definition "id_p \<equiv> Abs_p_set (Pair {id} id)"
+
+
+lemma set_of_id [simp]: "set_of (id_p) = {id}" 
+  apply (clarsimp simp: set_of_def id_p_def)
+  by (subst Abs_p_set_inverse; clarsimp)
+
+lemma point_of_id [simp]: "point_of (id_p) = id" 
+  apply (clarsimp simp: point_of_def id_p_def)
+  by (subst Abs_p_set_inverse; clarsimp)
+
+lemma p_set_eqI: "set_of A = set_of B \<Longrightarrow> point_of A = point_of B \<Longrightarrow> A = B"
+  by (metis Rep_p_set_inject domain_pair.expand point_of_def set_of_def)
+
+lemma point_in_set[simp]: "point_of S \<in> set_of S"
+  by (metis (mono_tags, lifting) Rep_p_set mem_Collect_eq point_of_def set_of_def)
+
+lemma id_in_set[simp]: "id \<in> set_of S"
+  by (metis (mono_tags, lifting) Rep_p_set mem_Collect_eq point_of_def set_of_def)
+
+definition "valid_dp S \<equiv> \<forall>f\<in>S. \<forall>g\<in>S. f o g = f" 
+
+lemma commutative_lens_get_set: "valid_lens b \<Longrightarrow> valid_lens c \<Longrightarrow> 
+      (\<lambda>s. set b s v) o (\<lambda>s. set c s v') = (\<lambda>s. set c s v') o (\<lambda>s. set b s v) \<Longrightarrow>
+          v = get b (set c (set b s v) v')"
+  by (metis comp_apply get_set_def valid_lens_def)
+
+lemma surj_setter: "valid_lens l \<Longrightarrow> surj (\<lambda>(s, v). set l s v)"
+  apply (clarsimp simp: surj_def)
+  by (metis set_get_def valid_lens_def)
+
+lemma lens_commuteI:  "valid_lens b \<Longrightarrow> valid_lens c \<Longrightarrow> 
+        ((\<lambda>s. set b s v) o (\<lambda>s. set c s v') = (\<lambda>s. set b s v) \<and> (\<lambda>s. set b s v) o (\<lambda>s. set c s v') = (\<lambda>s. set c s v')) \<or>
+      (\<forall>v v'. (\<lambda>s. set b s v) o (\<lambda>s. set c s v') = (\<lambda>s. set c s v') o (\<lambda>s. set b s v)) \<Longrightarrow> (\<lambda>s. set b s v) o (\<lambda>s. set c s v') = (\<lambda>s. set c s v') o (\<lambda>s. set b s v)"
+  apply (intro ext; clarsimp)
+  apply (elim disjE; clarsimp?)
+   apply metis
+  by (metis comp_apply)
+
+end
